Prove that the first conflicting element is in mo with another element
Prove that the first conflicting element is in mo with another
element. This commit also contains an interesting proof about
cycles of union.

exec.v
@@ -775,6 +775,32 @@ Proof.
   intuition (auto using (imm_rel_implies_rel (sb ex))).
 Qed.
 
+Lemma rmw_orig_read (x y: Event):
+  (rmw ex) x y ->
+  is_read x.
+Proof.
+  intros Hrmw.
+  destruct_val_exec val_exec.
+  destruct_rmw_v Hrmw_v.
+  apply Hrmw_vpairs in Hrmw as Hrmwp.
+  unfold valid_rmw_pair in Hrmwp.
+  destruct (get_mode x); destruct (get_mode y);
+  intuition auto.
+Qed.
+
+Lemma rmw_dest_write (x y: Event):
+  (rmw ex) x y ->
+  is_write y.
+Proof.
+  intros Hrmw.
+  destruct_val_exec val_exec.
+  destruct_rmw_v Hrmw_v.
+  apply Hrmw_vpairs in Hrmw as Hrmwp.
+  unfold valid_rmw_pair in Hrmwp.
+  destruct (get_mode x); destruct (get_mode y);
+  intuition auto.
+Qed.
+
 (** In a valid execution, events related by modification order belong to the set
 of events of the execution *)
 
@@ -855,7 +881,6 @@ Proof.
   auto.
 Qed.
 
-
 End ValidExecs.
   
 (** ** Getters *)
@@ -865,6 +890,12 @@ Definition reads (ex: Execution) : Ensemble Event :=
 
 Definition writes (ex: Execution) : Ensemble Event :=
   fun e => (In _ ex.(evts) e) /\ is_write e.
+
+(** Atomic events are events that are either in the domain or in the range of
+[rmw] *)
+
+Definition At (ex: Execution) : Ensemble Event :=
+  Union _ (dom ex.(rmw)) (ran ex.(rmw)).
 
 (** ** Completeness *)
 
